

Derivation of the Validation MSE and its Derivative w.r.t. λ

“All models are wrong, but some are useful.” — G. E. P. Box

1 Problem setup and notation

Let

- $N \in \mathbb{N}$ be the length of the time series.
- $\mathbf{Z} \in \mathbb{R}^N$ be the observed data vector:

$$\mathbf{Z} = \begin{bmatrix} Z_1 \\ Z_2 \\ \vdots \\ Z_N \end{bmatrix}.$$

- $d \in \mathbb{N}$ be the order of differencing used in the penalty.
- $K \in \mathbb{R}^{(N-d) \times N}$ be the differencing matrix of order d .
- $\lambda > 0$ be the smoothing (penalty) parameter.

We consider the penalized least squares problem

$$\min_{\mathbf{t} \in \mathbb{R}^N} J(\mathbf{t}; \lambda) := \|\mathbf{Z} - \mathbf{t}\|_2^2 + \lambda \|K\mathbf{t}\|_2^2. \quad (1)$$

The goal is:

- For each $\lambda > 0$, compute the trend estimator

$$\hat{\mathbf{t}}(\lambda) = \arg \min_{\mathbf{t}} J(\mathbf{t}; \lambda).$$

- On a separate validation set, define the mean squared error as a function of λ ,

$$f(\lambda) := \text{MSE}_{\text{val}}(\lambda),$$

and derive an explicit expression for the derivative $\frac{d}{d\lambda} f(\lambda)$.

2 Closed form of the penalized estimator

We solve (1) explicitly.

First note that

$$\|\mathbf{Z} - \mathbf{t}\|_2^2 = (\mathbf{Z} - \mathbf{t})^\top (\mathbf{Z} - \mathbf{t}), \quad \|K\mathbf{t}\|_2^2 = (K\mathbf{t})^\top (K\mathbf{t}).$$

Thus

$$\begin{aligned} J(\mathbf{t}; \lambda) &= (\mathbf{Z} - \mathbf{t})^\top (\mathbf{Z} - \mathbf{t}) + \lambda (K\mathbf{t})^\top (K\mathbf{t}) \\ &= (\mathbf{Z} - \mathbf{t})^\top (\mathbf{Z} - \mathbf{t}) + \lambda \mathbf{t}^\top K^\top K \mathbf{t}. \end{aligned}$$

Expand the first quadratic term:

$$(\mathbf{Z} - \mathbf{t})^\top (\mathbf{Z} - \mathbf{t}) = \mathbf{Z}^\top \mathbf{Z} - 2\mathbf{Z}^\top \mathbf{t} + \mathbf{t}^\top \mathbf{t}.$$

Hence

$$J(\mathbf{t}; \lambda) = \mathbf{Z}^\top \mathbf{Z} - 2\mathbf{Z}^\top \mathbf{t} + \mathbf{t}^\top \mathbf{t} + \lambda \mathbf{t}^\top K^\top K \mathbf{t}.$$

Group the terms that depend on \mathbf{t} :

$$\begin{aligned} J(\mathbf{t}; \lambda) &= \mathbf{Z}^\top \mathbf{Z} + \left(\mathbf{t}^\top \mathbf{t} + \lambda \mathbf{t}^\top K^\top K \mathbf{t} - 2\mathbf{Z}^\top \mathbf{t} \right) \\ &= \mathbf{Z}^\top \mathbf{Z} + \left(\mathbf{t}^\top (I_N + \lambda K^\top K) \mathbf{t} - 2\mathbf{Z}^\top \mathbf{t} \right), \end{aligned}$$

where I_N is the $N \times N$ identity matrix.

Define the symmetric positive definite matrix

$$A(\lambda) := I_N + \lambda K^\top K \in \mathbb{R}^{N \times N}.$$

Then

$$J(\mathbf{t}; \lambda) = \mathbf{Z}^\top \mathbf{Z} + \mathbf{t}^\top A(\lambda) \mathbf{t} - 2\mathbf{Z}^\top \mathbf{t}.$$

To find the minimizer, compute the gradient of J with respect to \mathbf{t} and set it equal to $\mathbf{0}$:

$$\nabla_{\mathbf{t}} J(\mathbf{t}; \lambda) = \mathbf{0}.$$

Recall:

- If A is symmetric, then $\nabla_{\mathbf{t}} (\mathbf{t}^\top A \mathbf{t}) = 2A\mathbf{t}$.
- $\nabla_{\mathbf{t}} (\mathbf{Z}^\top \mathbf{t}) = \mathbf{Z}$.

Apply this:

$$\begin{aligned}\nabla_{\mathbf{t}} J(\mathbf{t}; \lambda) &= \nabla_{\mathbf{t}} \left[\mathbf{Z}^\top \mathbf{Z} + \mathbf{t}^\top A(\lambda) \mathbf{t} - 2\mathbf{Z}^\top \mathbf{t} \right] \\ &= 0 + 2A(\lambda) \mathbf{t} - 2\mathbf{Z}.\end{aligned}$$

Set gradient equal to $\mathbf{0}$:

$$\begin{aligned}\nabla_{\mathbf{t}} J(\mathbf{t}; \lambda) = \mathbf{0} &\iff 2A(\lambda) \mathbf{t} - 2\mathbf{Z} = \mathbf{0} \\ &\iff 2A(\lambda) \mathbf{t} = 2\mathbf{Z} \\ &\iff A(\lambda) \mathbf{t} = \mathbf{Z}.\end{aligned}$$

Thus the minimizer solves the linear system

$$A(\lambda) \hat{\mathbf{t}}(\lambda) = \mathbf{Z}.$$

Since $A(\lambda)$ is symmetric positive definite, it is invertible, so

$$\hat{\mathbf{t}}(\lambda) = A(\lambda)^{-1} \mathbf{Z}. \quad (2)$$

Define the *smoothing matrix*

$$S(\lambda) := A(\lambda)^{-1} = (I_N + \lambda K^\top K)^{-1}.$$

Then

$$\hat{\mathbf{t}}(\lambda) = S(\lambda) \mathbf{Z}. \quad (3)$$

3 Validation set and validation MSE

Let $\mathcal{V} \subset \{1, 2, \dots, N\}$ denote the index set of validation observations, and let

$$n_{\text{val}} := |\mathcal{V}|$$

be the number of validation points.

Define the *selection matrix* $R \in \mathbb{R}^{n_{\text{val}} \times N}$ such that

$$\mathbf{Z}_{\text{val}} := R\mathbf{Z} \in \mathbb{R}^{n_{\text{val}}}$$

is the vector of validation observations. Concretely, each row of R is a standard basis vector selecting the corresponding index in \mathcal{V} .

Similarly, the fitted trend on the validation points is

$$\hat{\mathbf{t}}_{\text{val}}(\lambda) := R\hat{\mathbf{t}}(\lambda) = RS(\lambda) \mathbf{Z}.$$

Define the validation residual vector

$$\mathbf{r}(\lambda) := \mathbf{Z}_{\text{val}} - \hat{\mathbf{t}}_{\text{val}}(\lambda) = R\mathbf{Z} - RS(\lambda)\mathbf{Z}. \quad (4)$$

The validation mean squared error (MSE) as a function of λ is

$$f(\lambda) := \text{MSE}_{\text{val}}(\lambda) := \frac{1}{n_{\text{val}}} \|\mathbf{r}(\lambda)\|_2^2 = \frac{1}{n_{\text{val}}} \mathbf{r}(\lambda)^\top \mathbf{r}(\lambda). \quad (5)$$

Our objective is now:

$$\text{derive } \frac{d}{d\lambda} f(\lambda).$$

4 Mechanism: validation MSE $f(\lambda)$ and its derivative (slow version)

In this section we will go **very slowly**.

We want to compute the derivative of the validation MSE

$$f(\lambda) = \text{MSE}_{\text{val}}(\lambda)$$

with respect to the smoothing parameter λ .

We will do it in four steps:

1. Recall all the objects we already defined.
2. Compute the derivative of the smoothing matrix $S(\lambda)$.
3. Compute the derivative of the residual vector $\mathbf{r}(\lambda)$.
4. Use these to compute the derivative $f'(\lambda)$.

Throughout this section we will always write derivatives as

$$\frac{d}{d\lambda}(\cdot).$$

4.1 Step 1: Reminder of the objects

We have:

- The data vector $\mathbf{Z} \in \mathbb{R}^N$.
- The differencing matrix $K \in \mathbb{R}^{(N-d) \times N}$.
- The matrix

$$A(\lambda) := I_N + \lambda K^\top K \in \mathbb{R}^{N \times N}.$$

- The smoothing matrix

$$S(\lambda) := A(\lambda)^{-1} = (I_N + \lambda K^\top K)^{-1}.$$

- The fitted trend on all N points

$$\hat{\mathbf{t}}(\lambda) = S(\lambda)\mathbf{Z}.$$

- The validation selection matrix $R \in \mathbb{R}^{n_{\text{val}} \times N}$, which picks only the validation indices.

– Validation observations:

$$\mathbf{Z}_{\text{val}} = R\mathbf{Z}.$$

– Validation fitted trend:

$$\hat{\mathbf{t}}_{\text{val}}(\lambda) := R\hat{\mathbf{t}}(\lambda) = RS(\lambda)\mathbf{Z}.$$

- The validation residual vector:

$$\mathbf{r}(\lambda) := \mathbf{Z}_{\text{val}} - \hat{\mathbf{t}}_{\text{val}}(\lambda) = R\mathbf{Z} - RS(\lambda)\mathbf{Z}.$$

- The validation MSE:

$$f(\lambda) := \frac{1}{n_{\text{val}}} \|\mathbf{r}(\lambda)\|_2^2 = \frac{1}{n_{\text{val}}} \mathbf{r}(\lambda)^\top \mathbf{r}(\lambda). \quad (6)$$

Our goal is to compute

$$f'(\lambda) := \frac{d}{d\lambda} f(\lambda).$$

4.2 Step 2: Derivative of $S(\lambda) = A(\lambda)^{-1}$

First we compute the derivative of $A(\lambda)$.

Recall:

$$A(\lambda) = I_N + \lambda K^\top K.$$

We differentiate $A(\lambda)$ with respect to λ :

$$\begin{aligned} \frac{d}{d\lambda} A(\lambda) &= \frac{d}{d\lambda} (I_N + \lambda K^\top K) \\ &= \frac{d}{d\lambda} (I_N) + \frac{d}{d\lambda} (\lambda K^\top K). \end{aligned}$$

Now note:

- I_N does *not* depend on λ , so

$$\frac{d}{d\lambda} (I_N) = 0.$$

- For the term $\lambda K^\top K$, $K^\top K$ is constant and only λ varies. So

$$\frac{d}{d\lambda} (\lambda K^\top K) = 1 \cdot K^\top K.$$

Therefore

$$\frac{d}{d\lambda}A(\lambda) = K^\top K. \quad (7)$$

Now we use the matrix derivative formula for inverses. If $A(\lambda)$ is an invertible matrix depending on λ , then

$$\frac{d}{d\lambda}A(\lambda)^{-1} = -A(\lambda)^{-1} \left(\frac{d}{d\lambda}A(\lambda) \right) A(\lambda)^{-1}. \quad (8)$$

We apply (16) to $A(\lambda)$:

$$\begin{aligned} \frac{d}{d\lambda}S(\lambda) &= \frac{d}{d\lambda}A(\lambda)^{-1} \\ &= -A(\lambda)^{-1} \left(\frac{d}{d\lambda}A(\lambda) \right) A(\lambda)^{-1}. \end{aligned}$$

Replace $\frac{d}{d\lambda}A(\lambda)$ using (15) and $A(\lambda)^{-1} = S(\lambda)$:

$$\begin{aligned} \frac{d}{d\lambda}S(\lambda) &= -A(\lambda)^{-1}(K^\top K)A(\lambda)^{-1} \\ &= -S(\lambda)K^\top KS(\lambda). \end{aligned}$$

We write this more compactly as

$$S'(\lambda) := \frac{d}{d\lambda}S(\lambda) = -S(\lambda)K^\top KS(\lambda). \quad (9)$$

This is the key formula for the derivative of the smoothing matrix.

4.3 Step 3: Derivative of the residual vector $\mathbf{r}(\lambda)$

Now recall that

$$\mathbf{r}(\lambda) = R\mathbf{Z} - RS(\lambda)\mathbf{Z}.$$

We differentiate this with respect to λ .

$$\frac{d}{d\lambda}\mathbf{r}(\lambda) = \frac{d}{d\lambda}(R\mathbf{Z} - RS(\lambda)\mathbf{Z}).$$

We treat each term separately.

First term: $\frac{d}{d\lambda}(R\mathbf{Z})$.

- R is a fixed matrix (it does not depend on λ).
- \mathbf{Z} is a fixed vector (it does not depend on λ).

Therefore:

$$\frac{d}{d\lambda}(R\mathbf{Z}) = R \frac{d}{d\lambda}(\mathbf{Z}) = R \cdot \mathbf{0} = \mathbf{0}.$$

Second term: $\frac{d}{d\lambda}(RS(\lambda)\mathbf{Z})$. Again R and \mathbf{Z} are constants with respect to λ , so we only differentiate $S(\lambda)$:

$$\begin{aligned} \frac{d}{d\lambda}(RS(\lambda)\mathbf{Z}) &= R \frac{d}{d\lambda}(S(\lambda)\mathbf{Z}) \\ &= R(S'(\lambda)\mathbf{Z}). \end{aligned}$$

Putting both terms together:

$$\begin{aligned} \frac{d}{d\lambda}\mathbf{r}(\lambda) &= \frac{d}{d\lambda}(R\mathbf{Z}) - \frac{d}{d\lambda}(RS(\lambda)\mathbf{Z}) \\ &= \mathbf{0} - RS'(\lambda)\mathbf{Z} \\ &= -RS'(\lambda)\mathbf{Z}. \end{aligned}$$

Now substitute $S'(\lambda)$ from (17):

$$S'(\lambda) = -S(\lambda)K^\top KS(\lambda).$$

So

$$\begin{aligned} \frac{d}{d\lambda}\mathbf{r}(\lambda) &= -R(-S(\lambda)K^\top KS(\lambda))\mathbf{Z} \\ &= RS(\lambda)K^\top KS(\lambda)\mathbf{Z}. \end{aligned}$$

Therefore we define

$$\mathbf{r}'(\lambda) := \frac{d}{d\lambda}\mathbf{r}(\lambda) = RS(\lambda)K^\top KS(\lambda)\mathbf{Z}. \quad (10)$$

4.4 Step 4: Derivative of the validation MSE $f(\lambda)$

We start from the definition (14):

$$f(\lambda) = \frac{1}{n_{\text{val}}} \mathbf{r}(\lambda)^\top \mathbf{r}(\lambda).$$

To differentiate this, it is useful to first expand it as a sum over components.

Let

$$\mathbf{r}(\lambda) = \begin{bmatrix} r_1(\lambda) \\ r_2(\lambda) \\ \vdots \\ r_{n_{\text{val}}}(\lambda) \end{bmatrix} \in \mathbb{R}^{n_{\text{val}}}.$$

Then

$$\mathbf{r}(\lambda)^\top \mathbf{r}(\lambda) = \sum_{i=1}^{n_{\text{val}}} r_i(\lambda)^2,$$

so

$$f(\lambda) = \frac{1}{n_{\text{val}}} \sum_{i=1}^{n_{\text{val}}} r_i(\lambda)^2. \quad (11)$$

Now differentiate (19) with respect to λ , term by term:

$$\begin{aligned} \frac{d}{d\lambda} f(\lambda) &= \frac{d}{d\lambda} \left(\frac{1}{n_{\text{val}}} \sum_{i=1}^{n_{\text{val}}} r_i(\lambda)^2 \right) \\ &= \frac{1}{n_{\text{val}}} \sum_{i=1}^{n_{\text{val}}} \frac{d}{d\lambda} (r_i(\lambda)^2). \end{aligned}$$

Now use the usual scalar chain rule: for any scalar function $g(\lambda)$,

$$\frac{d}{d\lambda} (g(\lambda)^2) = 2g(\lambda)g'(\lambda).$$

Apply this with $g(\lambda) = r_i(\lambda)$:

$$\frac{d}{d\lambda} (r_i(\lambda)^2) = 2r_i(\lambda)r'_i(\lambda).$$

Therefore:

$$\begin{aligned}\frac{d}{d\lambda}f(\lambda) &= \frac{1}{n_{\text{val}}} \sum_{i=1}^{n_{\text{val}}} 2r_i(\lambda)r'_i(\lambda) \\ &= \frac{2}{n_{\text{val}}} \sum_{i=1}^{n_{\text{val}}} r_i(\lambda)r'_i(\lambda).\end{aligned}$$

Now we recognize the sum

$$\sum_{i=1}^{n_{\text{val}}} r_i(\lambda)r'_i(\lambda)$$

as the usual Euclidean inner product of the vectors

$$\mathbf{r}(\lambda) \quad \text{and} \quad \mathbf{r}'(\lambda).$$

Indeed,

$$\mathbf{r}(\lambda)^\top \mathbf{r}'(\lambda) = \sum_{i=1}^{n_{\text{val}}} r_i(\lambda)r'_i(\lambda).$$

Therefore we can rewrite the derivative as

$$f'(\lambda) := \frac{d}{d\lambda}f(\lambda) = \frac{2}{n_{\text{val}}} \mathbf{r}(\lambda)^\top \mathbf{r}'(\lambda). \quad (12)$$

Finally, we substitute the expressions for

$$\mathbf{r}(\lambda) = R\mathbf{Z} - RS(\lambda)\mathbf{Z} = R(I_N - S(\lambda))\mathbf{Z},$$

and for $\mathbf{r}'(\lambda)$ from (18),

$$\mathbf{r}'(\lambda) = RS(\lambda)K^\top KS(\lambda)\mathbf{Z}.$$

Thus

$$f'(\lambda) = \frac{2}{n_{\text{val}}} \left(R(I_N - S(\lambda))\mathbf{Z} \right)^\top \left(RS(\lambda)K^\top KS(\lambda)\mathbf{Z} \right).$$

So the final formula for the derivative of the validation MSE is

$$f'(\lambda) = \frac{2}{n_{\text{val}}} \left[R(I_N - S(\lambda))\mathbf{Z} \right]^\top \left[RS(\lambda)K^\top KS(\lambda)\mathbf{Z} \right], \quad S(\lambda) = (I_N + \lambda K^\top K)^{-1}.$$

(13)

5 Mechanism: validation MSE $f(\lambda)$ and its derivative (slow version)

In this section we will go **very slowly**.

We want to compute the derivative of the validation MSE

$$f(\lambda) = \text{MSE}_{\text{val}}(\lambda)$$

with respect to the smoothing parameter λ .

We will do it in four steps:

1. Recall all the objects we already defined.
2. Compute the derivative of the smoothing matrix $S(\lambda)$.
3. Compute the derivative of the residual vector $\mathbf{r}(\lambda)$.
4. Use these to compute the derivative $f'(\lambda)$.

Throughout this section we will always write derivatives as

$$\frac{d}{d\lambda}(\cdot).$$

5.1 Step 1: Reminder of the objects

We have:

- The data vector $\mathbf{Z} \in \mathbb{R}^N$.
- The differencing matrix $K \in \mathbb{R}^{(N-d) \times N}$.
- The matrix

$$A(\lambda) := I_N + \lambda K^\top K \in \mathbb{R}^{N \times N}.$$

- The smoothing matrix

$$S(\lambda) := A(\lambda)^{-1} = (I_N + \lambda K^\top K)^{-1}.$$

- The fitted trend on all N points

$$\hat{\mathbf{t}}(\lambda) = S(\lambda)\mathbf{Z}.$$

- The validation selection matrix $R \in \mathbb{R}^{n_{\text{val}} \times N}$, which picks only the validation indices.

– Validation observations:

$$\mathbf{Z}_{\text{val}} = R\mathbf{Z}.$$

– Validation fitted trend:

$$\hat{\mathbf{t}}_{\text{val}}(\lambda) := R\hat{\mathbf{t}}(\lambda) = RS(\lambda)\mathbf{Z}.$$

- The validation residual vector:

$$\mathbf{r}(\lambda) := \mathbf{Z}_{\text{val}} - \hat{\mathbf{t}}_{\text{val}}(\lambda) = R\mathbf{Z} - RS(\lambda)\mathbf{Z}.$$

- The validation MSE:

$$f(\lambda) := \frac{1}{n_{\text{val}}} \|\mathbf{r}(\lambda)\|_2^2 = \frac{1}{n_{\text{val}}} \mathbf{r}(\lambda)^\top \mathbf{r}(\lambda). \quad (14)$$

Our goal is to compute

$$f'(\lambda) := \frac{d}{d\lambda} f(\lambda).$$

5.2 Step 2: Derivative of $S(\lambda) = A(\lambda)^{-1}$

First we compute the derivative of $A(\lambda)$.

Recall:

$$A(\lambda) = I_N + \lambda K^\top K.$$

We differentiate $A(\lambda)$ with respect to λ :

$$\begin{aligned} \frac{d}{d\lambda} A(\lambda) &= \frac{d}{d\lambda} (I_N + \lambda K^\top K) \\ &= \frac{d}{d\lambda} (I_N) + \frac{d}{d\lambda} (\lambda K^\top K). \end{aligned}$$

Now note:

- I_N does *not* depend on λ , so

$$\frac{d}{d\lambda} (I_N) = 0.$$

- For the term $\lambda K^\top K$, $K^\top K$ is constant and only λ varies. So

$$\frac{d}{d\lambda} (\lambda K^\top K) = 1 \cdot K^\top K.$$

Therefore

$$\frac{d}{d\lambda}A(\lambda) = K^\top K. \quad (15)$$

Now we use the matrix derivative formula for inverses. If $A(\lambda)$ is an invertible matrix depending on λ , then

$$\frac{d}{d\lambda}A(\lambda)^{-1} = -A(\lambda)^{-1} \left(\frac{d}{d\lambda}A(\lambda) \right) A(\lambda)^{-1}. \quad (16)$$

We apply (16) to $A(\lambda)$:

$$\begin{aligned} \frac{d}{d\lambda}S(\lambda) &= \frac{d}{d\lambda}A(\lambda)^{-1} \\ &= -A(\lambda)^{-1} \left(\frac{d}{d\lambda}A(\lambda) \right) A(\lambda)^{-1}. \end{aligned}$$

Replace $\frac{d}{d\lambda}A(\lambda)$ using (15) and $A(\lambda)^{-1} = S(\lambda)$:

$$\begin{aligned} \frac{d}{d\lambda}S(\lambda) &= -A(\lambda)^{-1}(K^\top K)A(\lambda)^{-1} \\ &= -S(\lambda)K^\top KS(\lambda). \end{aligned}$$

We write this more compactly as

$$S'(\lambda) := \frac{d}{d\lambda}S(\lambda) = -S(\lambda)K^\top KS(\lambda). \quad (17)$$

This is the key formula for the derivative of the smoothing matrix.

5.3 Step 3: Derivative of the residual vector $\mathbf{r}(\lambda)$

Now recall that

$$\mathbf{r}(\lambda) = R\mathbf{Z} - RS(\lambda)\mathbf{Z}.$$

We differentiate this with respect to λ .

$$\frac{d}{d\lambda}\mathbf{r}(\lambda) = \frac{d}{d\lambda}(R\mathbf{Z} - RS(\lambda)\mathbf{Z}).$$

We treat each term separately.

First term: $\frac{d}{d\lambda}(R\mathbf{Z})$.

- R is a fixed matrix (it does not depend on λ).
- \mathbf{Z} is a fixed vector (it does not depend on λ).

Therefore:

$$\frac{d}{d\lambda}(R\mathbf{Z}) = R \frac{d}{d\lambda}(\mathbf{Z}) = R \cdot \mathbf{0} = \mathbf{0}.$$

Second term: $\frac{d}{d\lambda}(RS(\lambda)\mathbf{Z})$. Again R and \mathbf{Z} are constants with respect to λ , so we only differentiate $S(\lambda)$:

$$\begin{aligned} \frac{d}{d\lambda}(RS(\lambda)\mathbf{Z}) &= R \frac{d}{d\lambda}(S(\lambda)\mathbf{Z}) \\ &= R(S'(\lambda)\mathbf{Z}). \end{aligned}$$

Putting both terms together:

$$\begin{aligned} \frac{d}{d\lambda}\mathbf{r}(\lambda) &= \frac{d}{d\lambda}(R\mathbf{Z}) - \frac{d}{d\lambda}(RS(\lambda)\mathbf{Z}) \\ &= \mathbf{0} - RS'(\lambda)\mathbf{Z} \\ &= -RS'(\lambda)\mathbf{Z}. \end{aligned}$$

Now substitute $S'(\lambda)$ from (17):

$$S'(\lambda) = -S(\lambda)K^\top KS(\lambda).$$

So

$$\begin{aligned} \frac{d}{d\lambda}\mathbf{r}(\lambda) &= -R(-S(\lambda)K^\top KS(\lambda))\mathbf{Z} \\ &= RS(\lambda)K^\top KS(\lambda)\mathbf{Z}. \end{aligned}$$

Therefore we define

$$\mathbf{r}'(\lambda) := \frac{d}{d\lambda}\mathbf{r}(\lambda) = RS(\lambda)K^\top KS(\lambda)\mathbf{Z}. \quad (18)$$

5.4 Step 4: Derivative of the validation MSE $f(\lambda)$

We start from the definition (14):

$$f(\lambda) = \frac{1}{n_{\text{val}}} \mathbf{r}(\lambda)^\top \mathbf{r}(\lambda).$$

To differentiate this, it is useful to first expand it as a sum over components.

Let

$$\mathbf{r}(\lambda) = \begin{bmatrix} r_1(\lambda) \\ r_2(\lambda) \\ \vdots \\ r_{n_{\text{val}}}(\lambda) \end{bmatrix} \in \mathbb{R}^{n_{\text{val}}}.$$

Then

$$\mathbf{r}(\lambda)^\top \mathbf{r}(\lambda) = \sum_{i=1}^{n_{\text{val}}} r_i(\lambda)^2,$$

so

$$f(\lambda) = \frac{1}{n_{\text{val}}} \sum_{i=1}^{n_{\text{val}}} r_i(\lambda)^2. \quad (19)$$

Now differentiate (19) with respect to λ , term by term:

$$\begin{aligned} \frac{d}{d\lambda} f(\lambda) &= \frac{d}{d\lambda} \left(\frac{1}{n_{\text{val}}} \sum_{i=1}^{n_{\text{val}}} r_i(\lambda)^2 \right) \\ &= \frac{1}{n_{\text{val}}} \sum_{i=1}^{n_{\text{val}}} \frac{d}{d\lambda} (r_i(\lambda)^2). \end{aligned}$$

Now use the usual scalar chain rule: for any scalar function $g(\lambda)$,

$$\frac{d}{d\lambda} (g(\lambda)^2) = 2g(\lambda)g'(\lambda).$$

Apply this with $g(\lambda) = r_i(\lambda)$:

$$\frac{d}{d\lambda} (r_i(\lambda)^2) = 2r_i(\lambda) r'_i(\lambda).$$

Therefore:

$$\begin{aligned}\frac{d}{d\lambda}f(\lambda) &= \frac{1}{n_{\text{val}}} \sum_{i=1}^{n_{\text{val}}} 2r_i(\lambda)r'_i(\lambda) \\ &= \frac{2}{n_{\text{val}}} \sum_{i=1}^{n_{\text{val}}} r_i(\lambda)r'_i(\lambda).\end{aligned}$$

Now we recognize the sum

$$\sum_{i=1}^{n_{\text{val}}} r_i(\lambda)r'_i(\lambda)$$

as the usual Euclidean inner product of the vectors

$$\mathbf{r}(\lambda) \quad \text{and} \quad \mathbf{r}'(\lambda).$$

Indeed,

$$\mathbf{r}(\lambda)^\top \mathbf{r}'(\lambda) = \sum_{i=1}^{n_{\text{val}}} r_i(\lambda)r'_i(\lambda).$$

Therefore we can rewrite the derivative as

$$f'(\lambda) := \frac{d}{d\lambda}f(\lambda) = \frac{2}{n_{\text{val}}} \mathbf{r}(\lambda)^\top \mathbf{r}'(\lambda). \quad (20)$$

Finally, we substitute the expressions for

$$\mathbf{r}(\lambda) = R\mathbf{Z} - RS(\lambda)\mathbf{Z} = R(I_N - S(\lambda))\mathbf{Z},$$

and for $\mathbf{r}'(\lambda)$ from (18),

$$\mathbf{r}'(\lambda) = RS(\lambda)K^\top KS(\lambda)\mathbf{Z}.$$

Thus

$$f'(\lambda) = \frac{2}{n_{\text{val}}} \left(R(I_N - S(\lambda))\mathbf{Z} \right)^\top \left(RS(\lambda)K^\top KS(\lambda)\mathbf{Z} \right).$$

So the final formula for the derivative of the validation MSE is

$$f'(\lambda) = \frac{2}{n_{\text{val}}} [R(I_N - S(\lambda))\mathbf{Z}]^\top [RS(\lambda)K^\top KS(\lambda)\mathbf{Z}], \quad S(\lambda) = (I_N + \lambda K^\top K)^{-1}.$$

(21)

6 Derivative of the smoothing matrix $S(\lambda)$

Recall

$$S(\lambda) = A(\lambda)^{-1}, \quad A(\lambda) = I_N + \lambda K^\top K.$$

First compute the derivative of $A(\lambda)$:

$$\frac{d}{d\lambda} A(\lambda) = \frac{d}{d\lambda} (I_N + \lambda K^\top K) = \mathbf{0} + 1 \cdot K^\top K = K^\top K.$$

Now use the well-known formula for the derivative of an inverse:

$$\frac{d}{d\lambda} A(\lambda)^{-1} = -A(\lambda)^{-1} \left(\frac{d}{d\lambda} A(\lambda) \right) A(\lambda)^{-1}.$$

Apply this with $A(\lambda)$ above:

$$\begin{aligned} \frac{d}{d\lambda} S(\lambda) &= \frac{d}{d\lambda} A(\lambda)^{-1} \\ &= -A(\lambda)^{-1} (K^\top K) A(\lambda)^{-1} \\ &= -S(\lambda) K^\top K S(\lambda). \end{aligned}$$

Thus

$$S'(\lambda) := \frac{d}{d\lambda} S(\lambda) = -S(\lambda) K^\top K S(\lambda). \quad (22)$$

7 Derivative of the validation residual $\mathbf{r}(\lambda)$

From (4), we have

$$\mathbf{r}(\lambda) = R\mathbf{Z} - RS(\lambda)\mathbf{Z}.$$

Differentiate with respect to λ :

$$\begin{aligned} \frac{d}{d\lambda} \mathbf{r}(\lambda) &= \frac{d}{d\lambda} (R\mathbf{Z} - RS(\lambda)\mathbf{Z}) \\ &= \frac{d}{d\lambda} (R\mathbf{Z}) - \frac{d}{d\lambda} (RS(\lambda)\mathbf{Z}). \end{aligned}$$

Note:

- R does not depend on λ .
- \mathbf{Z} does not depend on λ .

Therefore

$$\frac{d}{d\lambda}(R\mathbf{Z}) = R \cdot \mathbf{0} = \mathbf{0}.$$

For the second term, treat R as constant and apply the chain rule:

$$\frac{d}{d\lambda}(RS(\lambda)\mathbf{Z}) = R\frac{d}{d\lambda}(S(\lambda)\mathbf{Z}).$$

Since \mathbf{Z} is constant, we differentiate $S(\lambda)$:

$$\frac{d}{d\lambda}(S(\lambda)\mathbf{Z}) = S'(\lambda)\mathbf{Z}.$$

Thus

$$\frac{d}{d\lambda}(RS(\lambda)\mathbf{Z}) = RS'(\lambda)\mathbf{Z}.$$

Combining both pieces:

$$\begin{aligned}\frac{d}{d\lambda}\mathbf{r}(\lambda) &= \mathbf{0} - RS'(\lambda)\mathbf{Z} \\ &= -RS'(\lambda)\mathbf{Z}.\end{aligned}$$

Now substitute $S'(\lambda)$ from (22):

$$S'(\lambda) = -S(\lambda)K^\top KS(\lambda).$$

Therefore

$$\begin{aligned}\frac{d}{d\lambda}\mathbf{r}(\lambda) &= -R\left(-S(\lambda)K^\top KS(\lambda)\right)\mathbf{Z} \\ &= RS(\lambda)K^\top KS(\lambda)\mathbf{Z}.\end{aligned}$$

So we have

$$\mathbf{r}'(\lambda) := \frac{d}{d\lambda}\mathbf{r}(\lambda) = RS(\lambda)K^\top KS(\lambda)\mathbf{Z}. \quad (23)$$

8 Derivative of the validation MSE $f(\lambda)$

Recall the definition from (5):

$$f(\lambda) = \frac{1}{n_{\text{val}}}\mathbf{r}(\lambda)^\top \mathbf{r}(\lambda).$$

Let us write explicitly:

$$f(\lambda) = \frac{1}{n_{\text{val}}}\sum_{i=1}^{n_{\text{val}}}r_i(\lambda)^2, \quad (24)$$

where $r_i(\lambda)$ is the i -th component of the vector $\mathbf{r}(\lambda)$.

8.1 Step-by-step scalar derivative

Differentiate (24) term by term:

$$\begin{aligned}\frac{d}{d\lambda}f(\lambda) &= \frac{d}{d\lambda} \left(\frac{1}{n_{\text{val}}} \sum_{i=1}^{n_{\text{val}}} r_i(\lambda)^2 \right) \\ &= \frac{1}{n_{\text{val}}} \sum_{i=1}^{n_{\text{val}}} \frac{d}{d\lambda} (r_i(\lambda)^2).\end{aligned}$$

For each i , apply the chain rule:

$$\frac{d}{d\lambda} (r_i(\lambda)^2) = 2r_i(\lambda) \cdot r'_i(\lambda).$$

Thus

$$\begin{aligned}\frac{d}{d\lambda}f(\lambda) &= \frac{1}{n_{\text{val}}} \sum_{i=1}^{n_{\text{val}}} 2r_i(\lambda)r'_i(\lambda) \\ &= \frac{2}{n_{\text{val}}} \sum_{i=1}^{n_{\text{val}}} r_i(\lambda)r'_i(\lambda).\end{aligned}$$

Now rewrite the sum as an inner product of vectors:

$$\sum_{i=1}^{n_{\text{val}}} r_i(\lambda)r'_i(\lambda) = \mathbf{r}(\lambda)^\top \mathbf{r}'(\lambda).$$

Therefore

$$f'(\lambda) := \frac{d}{d\lambda}f(\lambda) = \frac{2}{n_{\text{val}}} \mathbf{r}(\lambda)^\top \mathbf{r}'(\lambda). \quad (25)$$

8.2 Substituting $\mathbf{r}(\lambda)$ and $\mathbf{r}'(\lambda)$

From (4):

$$\mathbf{r}(\lambda) = R\mathbf{Z} - RS(\lambda)\mathbf{Z} = R(I_N - S(\lambda))\mathbf{Z}.$$

From (23):

$$\mathbf{r}'(\lambda) = RS(\lambda)K^\top KS(\lambda)\mathbf{Z}.$$

Substitute these into (25):

$$f'(\lambda) = \frac{2}{n_{\text{val}}} \left(R(I_N - S(\lambda))\mathbf{Z} \right)^\top \left(RS(\lambda)K^\top KS(\lambda)\mathbf{Z} \right).$$

Note that we cannot simplify much further in general, because R may not be square or symmetric. This is already a compact expression.

Hence the final expression for the derivative is

$$f'(\lambda) = \frac{2}{n_{\text{val}}} [R(I_N - S(\lambda))\mathbf{Z}]^\top [RS(\lambda)K^\top KS(\lambda)\mathbf{Z}]. \quad (26)$$

9 Special case: validation on all points

If the validation set is the entire sample, then $R = I_N$ and $n_{\text{val}} = N$.

In this case,

$$\mathbf{r}(\lambda) = (I_N - S(\lambda))\mathbf{Z},$$

and

$$\mathbf{r}'(\lambda) = S(\lambda)K^\top KS(\lambda)\mathbf{Z}.$$

Thus

$$\begin{aligned} f(\lambda) &= \frac{1}{N} \|(I_N - S(\lambda))\mathbf{Z}\|_2^2, \\ f'(\lambda) &= \frac{2}{N} [(I_N - S(\lambda))\mathbf{Z}]^\top [S(\lambda)K^\top KS(\lambda)\mathbf{Z}]. \end{aligned}$$

10 On solving $f'(\lambda) = 0$

To find the optimal λ^* that minimizes the validation MSE, one would like to solve

$$f'(\lambda^*) = 0.$$

However, even if we diagonalize

$$K^\top K = U\Lambda U^\top, \quad \Lambda = \text{diag}(\delta_1, \dots, \delta_N),$$

and write $S(\lambda) = (I + \lambda K^\top K)^{-1} = U(I + \lambda\Lambda)^{-1}U^\top$, the expression for $f(\lambda)$ becomes a sum of rational functions in λ of the form

$$\frac{(\text{polynomial in } \lambda)}{\prod_j (1 + \lambda\delta_j)^2},$$

and $f'(\lambda) = 0$ turns into a high-degree rational equation in λ with no general closed-form solution.

For this reason, in practice λ^* is found by one-dimensional numerical optimization (e.g., golden-section search, Brent's method, or Newton's method using $f'(\lambda)$ from (26)).

$$\frac{d}{d\lambda} \text{MSE}_{\text{val}}(\lambda) = \frac{2}{n_{\text{val}}} [R(I_N - S(\lambda))\mathbf{Z}]^\top \left[RS(\lambda)K^\top KS(\lambda)\mathbf{Z} \right], \quad S(\lambda) = (I_N + \lambda K^\top K)^{-1}.$$